changes

main.v
@@ -1,14 +1,19 @@
-Require Import String Arith List Lia Logic.
+Require Import String Arith List Lia.
 Import ListNotations.
-(* Open Scope string_scope. *)
+(* Require Import Program.
+Require Import Wf. *)
+Require Import Program.Wf.
 Module Part1.
-(* ToDo: Should Node be [Definition Node] or [Notation Node]? Check HW1 to see what I am talking about *)
+
+(* Representation of Graph *)
 Notation Node := nat.
 Definition Edge := (prod Node Node).
 Definition EdgeList := (list Edge).
 (* Type edge. *)
 Definition Graph := list (prod Node (list Node)).
+Definition EdgeGraph := list (prod Node Node).
 (* Definition Graph (n : Node) (edge_list : (list Edge) ) := list (prod Node (list Edge)). *)
+
 
 (* TODO := add the check to avoid duplicated edge addition *)
 Fixpoint add_edge (adj : Graph) (v1 v2: Node): Graph :=
@@ -80,6 +85,7 @@ Qed.
 
     
 
+(* The following functions retreives the union of parents and children nodes. *)
 Fixpoint get_all_neighbors (g: Graph) (u : Node): (list Node):=
     match g with
     | nil => nil
@@ -93,14 +99,15 @@ Fixpoint get_all_neighbors (g: Graph) (u : Node): (list Node):=
                     else n1
     end.
 
-Fixpoint get_actual_neighbors (g: Graph) (u : Node): (list Node):=
+(* The following functions only retreives the children nodes. *)
+Fixpoint get_children (g: Graph) (u : Node): (list Node):=
     match g with
     | nil => nil
     | (v,e)::g1 => 
                 if (Nat.eqb u v) 
                     then e 
                 else
-                    get_actual_neighbors g1 u
+                get_children g1 u
     end.
 
 
@@ -111,13 +118,13 @@ Proof.
 Qed.
 
 Example actual_nghbrs_of_1_in_one_line:
-    get_actual_neighbors one_line 1 = [2].
+    get_children one_line 1 = [2].
 Proof.
     simpl. auto.
 Qed.
 
 Example actual_nghbrs_of_2_in_one_line:
-    get_actual_neighbors one_line 2 = nil.
+    get_children one_line 2 = nil.
 Proof.
     simpl. auto.
 Qed.
@@ -157,25 +164,17 @@ Proof.
     simpl. auto.
 Qed.
 
-(* Fixpoint is_reachable_in_k_steps (u v: Node) (k: nat): Prop :=
-    match k with
-    | 0 => if (Nat.eqb u v) then True else False
-    | S => 
-Fixpoint get_reachable_nodes_helper (g:Graph) (list_u: list Node) (list_seen : list Node): (list Node) :=
-    match list_u with 
-    | nil => nil
-    | v::l => if (existsb (Nat.eqb v) list_seen)
-                    then (get_reachable_nodes_helper g l list_seen)
-                else v::(get_reachable_nodes_helper g ((get_actual_neighbors g v) ++ l ) (v::list_seen))
-    end.
-
-Fixpoint is_cyclic_direc (g: Graph) : Prop := *)
-
 Definition node_in (g: Graph) (n : Node) : Prop :=
     exists edge_list, In (n, edge_list) g.
 
 Example one_in_one_line:
     node_in one_line 1.
+Proof.
+    simpl. unfold node_in. unfold one_line. simpl. eauto.
+Qed.
+
+Example two_in_one_line:
+    node_in one_line 2.
 Proof.
     simpl. unfold node_in. unfold one_line. simpl. eauto.
 Qed.
@@ -188,7 +187,7 @@ Qed.
 
 (* RETURNS True if u->v in the graph g *)
 Definition edge_in (g: Graph) (u : Node) (v : Node) : Prop :=
-    forall ngbhrs_list, In (u, ngbhrs_list) g  ->  In v ngbhrs_list.
+    node_in g u /\ (forall ngbhrs_list,  (In (u, ngbhrs_list) g  ->  In v ngbhrs_list)).
 
 (* g = [(1, [2,3,4]), (3, [4,5])] *)
 (* g = [(1, [2,3,4]), (3, [4,5]), (1, [5])]  -- this does not exist in our exmaplewas*) 
@@ -201,7 +200,7 @@ Example one_two_in_one_line:
     edge_in one_line 1 2.
 Proof.
     (* simpl. unfold edge_in. unfold one_line. simpl. intros. split. destruct (1, edge_list). inversion H. easy. inversion H0. inversion H1. apply in_eq. easy.  *)
-    simpl. unfold edge_in. unfold one_line. simpl. intros. inversion H. easy. inversion H0. inversion H1. apply in_eq. easy. 
+    simpl. unfold edge_in. simpl. intros. split. apply one_in_one_line.  intros. inversion H. easy. inversion H0. inversion H1. apply in_eq. easy. 
 Qed.
 
 Example two_one_not_in_one_line:
@@ -210,16 +209,58 @@ Proof.
     intros .
     unfold edge_in in H.
     unfold one_line in H.
-    simpl in H.
-    specialize (H []).
+    simpl in H. destruct H. 
+    specialize (H0 []).
     firstorder.
 Qed.
 
 Example one_three_not_in_one_line:
     edge_in one_line 1 3 -> False.
 Proof.
-    unfold not. simpl. unfold edge_in. unfold one_line. simpl. intros. eauto. specialize (H [2]). firstorder. easy.
+    unfold not. simpl. unfold edge_in. unfold one_line. simpl. intros. destruct H. eauto. specialize (H0 [2]). firstorder. lia. easy.
 Qed.
+
+Fixpoint adj_graph_to_edge_list_helper (u: Node) (edge_list: list Node): EdgeGraph := 
+    match edge_list with 
+    | nil => nil
+    | (cons v edge_list_rest) => (u,v)::(adj_graph_to_edge_list_helper u edge_list_rest)
+    end.
+
+Fixpoint adj_graph_to_edge_list (graph: Graph): EdgeGraph := 
+    match graph with 
+    | nil => nil
+    | (cons (u,edge_list) rest_adj) => ((adj_graph_to_edge_list_helper u edge_list) ++ (adj_graph_to_edge_list rest_adj))
+    end.
+
+Compute adj_graph_to_edge_list [(1,[2;3;4]);(2,[3;4])].
+Lemma adj_reprsn_has_edge_list_reprsn: 
+    forall adj_graph, (exists edge_graph, (forall u v , edge_in adj_graph u v -> In (u, v) edge_graph)).
+Proof.
+intros.
+(* exists (adj_graph_to_edge_list adj_graph). *)
+intros.
+induction adj_graph.
+- exists (adj_graph_to_edge_list []). simpl. unfold edge_in. intros. destruct H. inversion H. firstorder.
+- exists (let (u, edge_list):=a in (adj_graph_to_edge_list_helper u edge_list) ++ (adj_graph_to_edge_list adj_graph)). intros. destruct a. eapply in_app_iff. inversion H; subst; clear H. inversion H0; subst; clear H0. inversion H. inversion H0; subst; clear H0.
+Admitted.
+
+Compute max 2 3.
+Fixpoint max_vertex (graph: EdgeGraph): Node :=
+    match graph with
+    | nil => 0
+    | (u,v)::rest_edge_list => max u (max v (max_vertex rest_edge_list)) 
+    end.
+
+Compute max_vertex [(1,2);(2,4);(4,5);(1,3)].
+
+Definition edge_list_to_adj_graph (graph: EdgeGraph): Graph := 
+    construct_dir_graph (max_vertex graph) graph.
+
+Lemma edge_reprsn_has_adj_graph_reprsn: 
+    forall edge_graph, (exists adj_graph, (forall u v , In (u, v) edge_graph -> edge_in adj_graph u v)).
+Proof.
+Admitted.
+
 
 
 Inductive is_reachable_ind : Graph -> Node -> Node -> Prop :=
@@ -269,43 +310,386 @@ Qed.
 
 
 
-Definition is_cyclic_ind (g: Graph) : Prop :=
-    exists v, node_in g v /\ is_reachable_ind g v v.
-    (* The following does not work because false is difficult to prove *)
-    (* exists v, node_in g v -> is_reachable_ind g v v. *)
 
-Example one_line_is_not_cyclic:
-    ~ (is_cyclic_ind one_line).
+
+(* ----------------------------------------------------------------------- *)
+
+(* Size of the Graph: Number of Nodes in the Graph *)
+Fixpoint get_size (g : Graph) : nat :=
+  match g with
+  | nil => 0
+  | (v, _) :: g' => 1 + get_size g'
+  end.
+Definition example_graph1 := construct_dir_graph 3 [(1, 2); (1, 3); (2, 1); (2, 3)]. 
+Example example_graph1_size : get_size example_graph1 = 3.
+Proof. reflexivity. Qed.
+  
+Definition example_graph2 := construct_dir_graph 2 [(1, 2)].
+Example example_graph2_size : get_size example_graph2 = 2.
+Proof. reflexivity. Qed.
+
+(* Non Connected graph *)
+Definition example_graph3 := construct_dir_graph 3 [(2, 3)].
+Example example_graph3_size : get_size example_graph3 = 3.
+Proof. reflexivity. Qed.
+
+Definition example_graph4: Graph := nil.
+Example example_graph4_size : get_size example_graph4 = 0.
+Proof. reflexivity. Qed.
+
+(* Implementing degrees of vertices *)
+Fixpoint degree (g : Graph) (v : Node) : nat :=
+  match g with
+  | [] => 0
+  | (u, neighbors) :: rest =>
+    if Nat.eqb u v then length neighbors
+    else degree rest v
+  end.
+
+(* Some example *)
+Example degree_example_1 : degree [(1, [2; 3]); (2, [1; 3]); (3, [1; 2])] 1 = 2.
 Proof.
-    unfold is_cyclic_ind. unfold not. firstorder. inversion H; subst; clear H. apply two_two_not_reachable_ind_in_one_line in H0. firstorder. inversion H; subst; clear H. apply one_one_not_reachable_ind_in_one_line in H0. firstorder.
+    reflexivity.
+Qed.
+
+Example degree_example_2 : degree [(1, [2; 3]); (2, [1; 3; 4; 5]); (3, [1; 2])] 2 = 4.
+Proof.
+    reflexivity.
+Qed.
+
+(* Lemma: Degree of vertices of an empty graph is always 0 *)
+Lemma degree_empty_graph : forall v, degree [] v = 0.
+Proof.
+    intros v. reflexivity.
+Qed.
+
+(* Lemma: Degree of vertices of a single vertex is always 0 *)
+Lemma degree_single_vertex : forall v u, v <> u -> degree [(u, [])] v = 0.
+Proof.
+    intros v u H. 
+    simpl.
+    destruct (Nat.eqb_spec u v).
+    - auto.
+    - auto.
+Qed.
+
+(* Lemma: Degree of vertices is always positive *)
+Lemma degree_positive : forall g v,
+  0 <= degree g v.
+Proof.
+    intros.
+    induction g.
+    - simpl. lia.
+    - simpl. destruct a as[u neighbors].
+        * apply Nat.le_0_l.     
 Qed.
 
 
-Example one_cycle_is_cyclic:
-    is_cyclic_ind one_cycle.
+(* The degree of vertices of a graph increases when we add an edge *)
+Lemma degree_add_edge : forall g v1 v2,
+  (* In v (fst (split g)) -> *)
+  (~ In v2 (get_children g v1)) -> degree (add_edge g v1 v2) v1 = S (degree g v1).
 Proof.
-    exists 1. split. 
-    unfold node_in. unfold one_cycle. simpl. exists [2]. firstorder.
-    apply one_one_reachable_in_one_cycle.
+    intros.
+    destruct H. destruct get_children.
+    - simpl. 
+
+Admitted.
+
+(* Property of Graph: The sum of degrees in an undirected graph equals twice the number of edges *)
+
+(* Helper to get sum of degrees in a graph *)
+Fixpoint sum_of_degrees_undirected (g : Graph) : nat :=
+  match g with
+  | [] => 0
+  | (n, adj) :: rest => length adj + sum_of_degrees_undirected rest
+  end.
+(* Helper to get number of edges in a graph *)
+Fixpoint num_edges (g : Graph) : nat :=
+  match g with
+  | [] => 0
+  | (n, adj) :: rest => length adj + num_edges rest
+  end.
+Definition num_edges_undirected (g : Graph) : nat :=
+    num_edges g / 2.
+
+Definition example_complex_undir_graph := 
+  construct_undir_graph 4 [(1, 2); (1, 3); (2, 3); (2, 4); (3, 4)].
+(* Compute(sum_of_degrees_undirected example_complex_undir_graph).
+Compute(num_edges_undirected example_complex_undir_graph). *)
+
+Theorem sum_of_degrees_equals_twice_edges : forall (g : Graph), 
+    sum_of_degrees_undirected g = 2 * num_edges_undirected g.
+Proof.
+  intros.
+  induction g.
+  - simpl. reflexivity.
+  - simpl. unfold num_edges_undirected in *. rewrite IHg.
+    destruct num_edges.
+    * simpl. 
+   (* unfold sum_of_degrees_undirected in *. *)
+    (* rewrite Nat.mul_add_distr_l. *)
+    (* unfold num_edges in *. simpl in IHg. rewrite IHg. 
+    rewrite Nat.div_add_l.
+    + reflexivity.
+    + apply Nat.neq_succ_0.
+      apply Nat.lt_0_succ. *)
+Admitted.
+
+(* ----------------------------------------------------------------------- *)
+
+(* For Directed Graphs: In-degree and Out-degree *)
+
+Fixpoint in_degree (g : Graph) (v : Node) : nat :=
+  match g with
+  | [] => 0
+  | (_, adj) :: rest => (if Nat.eq_dec (length (filter (Nat.eqb v) adj)) 0 then 0 else 1) + in_degree rest v
+  end.
+
+Fixpoint out_degree (g : Graph) (v : Node) : nat :=
+  match g with
+  | [] => 0
+  | (n, adj) :: rest => if Nat.eqb n v then length adj else out_degree rest v
+  end.
+
+Definition example_dir_graph1 := construct_dir_graph 4 [(1, 2); (1, 3); (2, 3); (3, 4)].
+Definition example_dir_graph2 := construct_dir_graph 5 [(1, 2); (1, 3); (2, 4); (3, 4); (4, 5)].
+
+Example in_degree_example_dir_graph1:
+  in_degree example_dir_graph1 3 = 2.
+Proof. reflexivity. Qed.
+
+Example out_degree_example_dir_graph1:
+  out_degree example_dir_graph1 1 = 2.
+Proof. reflexivity. Qed.
+
+Example in_degree_example_dir_graph_2:
+  in_degree example_dir_graph2 4 = 2.
+Proof. reflexivity. Qed.
+
+Example out_degree_example_dir_graph_2:
+  out_degree example_dir_graph2 4 = 1.
+Proof. reflexivity. Qed.
+
+(* Definition sum_in_degree (g : Graph) : nat := 
+Definition sum_out_degree (g : Graph) : nat := 
+Lemma sum_in_out_degrees_equal : forall g, forall v,
+  sum_in_degree g = sum_out_degree g.
+Proof.
+Admitted. *)
+
+(* Property: Sum of in_degrees out_degs is even *)
+Definition even_sum_degrees_property (g : Graph) : Prop :=
+  forall v, (in_degree g v + out_degree g v) mod 2 = 0.
+
+(* Proof Property *)
+Lemma even_sum_degrees_directed_graph : forall g : Graph,
+  even_sum_degrees_property g.
+Proof.
+  intros.
+  unfold even_sum_degrees_property.
+  induction g. simpl. 
+  - reflexivity.
+  - intros v. unfold in_degree in *. unfold out_degree in *.
+    simpl. destruct a.
+    (* simpl. rewrite IHg.  *)
+  
+  destruct (Nat.eq_dec n v) eqn:Eqn.
+    + subst.
+      (* apply IHg.
+    + apply IHg. *)
+Admitted.
+
+
+(* 
+    BFS Algorithm and reachability
+*)
+
+Fixpoint bfs_helper (g : Graph) (queue :  list Node) (visited : list Node)
+     (termination_counter : nat) : list Node :=
+    match termination_counter with
+    | O => rev visited
+    | S n =>
+        match queue with
+            | [] => rev visited
+            | cur :: queue' =>
+                if existsb (Nat.eqb cur) visited then bfs_helper g queue' visited n
+                else 
+                let neighbors := get_children g cur in
+                let queue'' := queue' ++ neighbors in
+                bfs_helper g queue'' (cur :: visited) n
+        end
+end.
+
+Definition bfs (g : Graph) (source : Node) : list Node :=
+    bfs_helper g [source] [] (get_size(g) * get_size(g)).
+
+Definition example_bfs_graph : Graph := construct_dir_graph 5 [(1, 2); (1, 3); (2, 4); (3, 2); (3, 5); (4, 5)].
+
+(*                    Example Graph
+      1 --> 2 --> 4
+      |     ^     |
+      |     |     v
+       ---> 3 --> 5
+*)
+
+Lemma bfs_one_visits_one:
+    In 1 (bfs example_bfs_graph 1).
+Proof.
+    simpl. lia.
 Qed.
 
-Definition is_dag (g:Graph) : Prop :=
-    is_cyclic_ind g -> False.
-
-
-
-Definition no_parent (g:Graph) (v:Node) : Prop :=
-    forall v1, node_in g v1 -> ~ edge_in g v1 v.
-
-Example one_has_noparent_in_one_line:
-    no_parent one_line 1.
+Lemma bfs_one_visits_four:
+    In 4 (bfs example_bfs_graph 1).
 Proof.
-    unfold no_parent. firstorder. inversion H; subst; clear H. unfold not. intros. unfold one_line in H. unfold edge_in in H. simpl in H. specialize (H []). firstorder.
-    inversion H; subst; clear H.
-    unfold not. intros. unfold one_line in H. unfold edge_in in H. simpl in H. specialize (H [2]). firstorder. easy.
+    simpl. lia.
 Qed.
 
+Lemma bfs_three_does_not_visit_one:
+    ~ In 1 (bfs example_bfs_graph 3).
+Proof.
+    simpl. unfold not. intros. 
+    destruct H. lia.
+    destruct H. lia.
+    destruct H. lia.
+    destruct H. lia.
+    destruct H.
+Qed.
 
+(* see other way: bool*)
+(* Fixpoint Unique (l : list Node) : Prop :=
+  match l with
+  | [] => True
+  | x :: xs => ~ In x xs /\ Unique xs
+  end. *)
+(* Trying to implement as a bool so easier to proove in Coq*)
+Fixpoint Unique (l : list Node) : bool :=
+match l with
+  | [] => true
+  | x :: xs => if existsb (Nat.eqb x) xs then false else Unique xs
+end.
+
+
+Lemma bfs_unique_visited : forall (g : Graph) (source : Node),
+    Unique (bfs g source) = true.
+Proof.
+  intros g source.
+  unfold Unique.
+  induction (bfs g source).
+  - auto.
+  - destruct (existsb (Nat.eqb a) l) eqn:Heq_existsb.
+    * apply existsb_exists in Heq_existsb.
+      destruct Heq_existsb as [x [Heq_x Hin_x]].
+      apply Nat.eqb_eq in Hin_x.
+      (* contradiction.
+      rewrite Heq_x in Hin_x.
+  fold Unique in *. eauto.  *)
+  (* split.
+    * induction l.
+      ** simpl. auto.
+      ** simpl. intros [Heq | Hin].
+        *** rewrite Heq in IHl. unfold Unique in IHl. eauto.  
+        admit.
+        *** fold Unique in IHl0. fold Unique in IHl.  admit.
+    * apply IHl. *)
+Admitted.
+
+Lemma bfs_terminates : forall (g : Graph) (source : Node),
+  exists nodes : list Node, bfs g source = nodes.
+Proof.
+  intros. unfold bfs.
+  induction (get_size g).
+  - exists []. reflexivity.
+  - simpl.
+Admitted.
+  
+Lemma bfs_never_more_than_size : forall (g: Graph) (source : Node), 
+  (get_size g >= 1) -> (get_size g) >= length (bfs g source).
+Proof.
+  intros.
+  induction bfs.
+  - simpl. lia.
+  - destruct l.
+    * apply H.
+    (* * eassumption. rewrite <- IHl.   *)
+Admitted.
+
+
+(* Function to get all pairs of nodes *)
+Fixpoint all_pairs (l : list Node) : list (Node * Node) :=
+  match l with
+  | nil => nil
+  | x :: xs => map (pair x) xs ++ all_pairs xs
+  end.
+
+  Example example_1: all_pairs [1; 2; 3] = [(1, 2); (1, 3); (2, 3)].
+  Proof. reflexivity. Qed.
+  
+  Example example_2: all_pairs [4; 5] = [(4, 5)].
+  Proof. reflexivity. Qed.
+  
+  Example example_3: all_pairs [6] = [].
+  Proof. reflexivity. Qed.
+
+(* Shortest Path Definition *)
+  Fixpoint shortest_path_helper (g: Graph) (srcs : list Node) (dst: Node) (visited: list Node) (fuel: nat): list Node  :=
+  match fuel with
+  | 0 => []
+  | S fuel' =>
+    match srcs with
+    | [] => []
+    | src :: xsrcs => (
+        let min_rest_path := (shortest_path_helper g xsrcs dst visited fuel') in
+        let curr_path := src::(shortest_path_helper g (get_children g src) dst (src::visited) fuel') in
+        if (Nat.eqb src dst) then
+            [src]
+        else if (existsb (Nat.eqb src) visited) then
+            min_rest_path
+        else if (Nat.eqb (length min_rest_path) 0) then
+            curr_path
+        else if (Nat.leb (length min_rest_path) (length curr_path)) then
+            min_rest_path
+        else
+            curr_path
+    )
+    end
+  end.
+
+Definition shortest_path (g: Graph) (src: Node) (dst: Node) : list Node :=
+    let path := (shortest_path_helper g [src] dst [] ((length g)*(length g))) in
+    match rev path with 
+    | v::l => if (Nat.eqb v dst) then   
+                path
+              else  
+                []
+    | _ => []
+    end.
+
+(* 
+    TO Calculate the DIAMETER of the graph 
+    We just assume that the diameter will be calculated only for connected graphs. ??
+    Diameter = longest shortest path between any 2 pair of nodes
+    - need the shortest distance between all pair of nodes
+    - Then need the max value among all those
+*)
+
+Definition diameter (g : Graph) : nat :=
+  let all_nodes := seq 1 (length g) in (* This can be done using a better helper function*)
+  let pairs := all_pairs all_nodes in
+  let diameters := map (fun '(src, dst) => length (shortest_path g src dst)) pairs in
+  fold_right max 0 diameters.
+
+(* Some Examples for Diameter *)
+Definition example_diameter_graph : Graph := construct_dir_graph 7 [(1, 2); (2, 3); (2, 4); (2, 5); (2, 6); (6, 7)].
+
+Example diameter_longest_path : 
+ diameter example_diameter_graph = 3. 
+Proof. reflexivity. Qed.
+
+
+(* Additional Properties and some extensions for Graph *)
+
+(* Walk in a graph *)   
 Inductive is_walk: Graph -> list Node -> Prop :=
 | walkOne : forall  g v, node_in g v -> is_walk g [v]
 | walkOneStep : forall g u v l, edge_in g u v -> is_walk g (v::l) -> is_walk g (u :: v :: l).
@@ -320,6 +704,7 @@ Fixpoint tail_elem (l : list Node) :=
   | [x] => Some x
   | _ :: xs => tail_elem xs
   end.
+
 
 Goal tail_elem [2;3;4] = Some 4.
 Proof.
@@ -342,42 +727,137 @@ Goal head_tail_same [1;2;1].
 Proof.
 eapply nonEmptyHeadTailSame. *)
 
+Fixpoint has_duplicates (l:list Node): Prop :=
+    match l with 
+    | nil => False
+    | a::l1 => In a l1 \/ (has_duplicates l1)
+    end.
+
+    Goal not (has_duplicates [1;2;3]).
+    Proof.
+    unfold not. firstorder. easy. easy. easy.
+    Qed.
+    
+    Goal has_duplicates [1;2;1;3].
+    Proof.
+    firstorder. 
+    Qed.
+    
+        
 
 Definition head_tail_same (l : list Node) :=
-    length l >= 2 /\ ((head l) = (tail_elem l)).
+    (length l >=2) /\ (head l) = (tail_elem l).
 
-Goal head_tail_same [2;3;2].
-Proof.
-unfold head_tail_same. split. unfold length. lia. firstorder.
-Qed.
-
+    Goal head_tail_same [2;3;2].
+    Proof.
+    firstorder. simpl. lia.
+    Qed.
     
+    Goal not (head_tail_same [2]).
+    Proof.
+    unfold head_tail_same. firstorder. simpl. lia.
+    Qed.
+
+    Goal not( head_tail_same []).
+    Proof.
+    unfold not. unfold head_tail_same. firstorder. simpl in H. lia.
+    Qed.
+
+            
 Definition is_path (g:Graph) (l: list Node) : Prop :=
-    is_walk g l /\ has_no_duplicates l.
+    is_walk g l /\ (not (has_duplicates l)).
 
 
 Definition is_cycle (g:Graph) (l: list Node) : Prop :=
-        is_walk g l /\ head_tail_same l.
+        length l>=2 /\ is_walk g l /\ head_tail_same l.
 
 Lemma head_tail_same_implies_duplicates:
-    forall l, head_tail_same l -> not ( has_no_duplicates l).
+    forall l, head_tail_same l -> has_duplicates l.
 Proof.
+intros. inversion H; subst;clear H. 
+(* assert (exists a l1, a::l1=l). inversion H0. inversion H2. 
 induction l.
-- unfold head_tail_same. intros. destruct H. simpl in H. firstorder. easy.
--intros. destruct H. 
+- unfold head_tail_same. intros. simpl in H. firstorder. easy.
+- intros. firstorder. simpl in H. inversion H; subst; clear H. destruct l. simpl in H. lia. simpl in H1. assert (In a (n::l)). simpl in H0.  *)
 Admitted.
+
 
 Lemma path_is_not_cycle: 
     forall g l, is_path g l -> not (is_cycle g l).
 Proof.
-    (* induction l.
-    - unfold not. intros. inversion H; subst; clear H. inversion H0; subst; clear H0. unfold head_tail_same in H3. inversion H3. simpl in H0. lia.
-    - intros. unfold not.  intros. inversion H . eapply walkOneStep in H1. inversion H2. simpl in H. *)
-    intros. unfold not, is_path, is_cycle. destruct H. intros. destruct H1. eapply head_tail_same_implies_duplicates in H0. easy. easy.
+    intros. unfold not, is_path, is_cycle. destruct H. intros. destruct H1. destruct H2. apply head_tail_same_implies_duplicates in H3. contradiction.
+Qed.
+Lemma cycle_is_not_path: 
+    forall g l, is_cycle g l -> not (is_path g l).
+Proof.
+    intros. unfold not, is_path, is_cycle. destruct H. intros. destruct H1. destruct H0. apply head_tail_same_implies_duplicates in H3. contradiction.
 Qed.
 
+
+Definition is_reachable_walk (g:Graph) (u:Node) (v:Node): Prop :=
+ exists walk, (length walk >=2) /\ is_walk g walk /\ ((head walk) = Some u) /\ ((tail_elem walk) = Some v).
+
+Definition is_cyclic (g: Graph) : Prop :=
+    exists l, is_cycle g l.
+    (* The following does not work because false is difficult to prove *)
+    (* exists v, node_in g v -> is_reachable_ind g v v. *)
+
+Definition is_dag (g:Graph) : Prop :=
+    is_cyclic g -> False.
+
+Lemma in_dag_no_node_is_reachable_to_itself:
+    forall g v, is_dag g -> node_in g v -> (not (is_reachable_walk g v v)).
+Proof.
+intros. unfold not. firstorder. (*Assuming a walk exists that starts and ends at the same node*)
+ assert (is_cycle g x). firstorder. rewrite H4. firstorder. (* Proving that the walk should be a cycle*)  
+ specialize (H x). simpl in H. firstorder. (*Proving that presence of a cylce contradicts that the graph is a DAG*)
+Qed. 
+    
+(* Lemma no_node_is_reachable_to_itself_implies_dag:
+    forall g v, node_in g v /\ (not (is_reachable_walk g v v)) -> is_dag g.
+Proof.
+ unfold is_dag.  firstorder. specialize (H1 x0). simpl in H1. firstorder. destruct H1. destruct x0. easy. simpl. inversion H2. easy. (*Assuming a walk exists that starts and ends at the same node*)
+ assert (is_cycle g x). firstorder. rewrite H4. firstorder. (* Proving that the walk should be a cycle*)  
+ specialize (H x). simpl in H. firstorder. (*Proving that presence of a cylce contradicts that the graph is a DAG*)
+Qed.  *)
+
+(* Example one_line_is_not_cyclic:
+    ~ (is_cyclic one_line).
+Proof.
+    unfold is_cyclic. unfold not. firstorder. inversion H; subst; clear H. apply two_two_not_reachable_ind_in_one_line in H0. firstorder. inversion H; subst; clear H. apply one_one_not_reachable_ind_in_one_line in H0. firstorder.
+Qed. *)
+
+
+Example one_cycle_is_cyclic:
+    is_cyclic one_cycle.
+Proof.
+    unfold is_cyclic. exists [1;2;1]. firstorder. simpl. lia. eapply walkOneStep. firstorder. unfold one_cycle. simpl. unfold node_in. exists [2]. firstorder.
+    inversion H. inversion H. firstorder.
+    eapply walkOneStep. firstorder. unfold one_cycle. simpl. unfold node_in. exists [1]. firstorder.
+    inversion H. inversion H. firstorder.
+    inversion H. eapply walkOne. unfold one_cycle. simpl. unfold node_in. exists [2]. firstorder. simpl. lia.
+Qed.
+
+
+
+
+Definition no_parent (g:Graph) (v:Node) : Prop :=
+    forall v1, node_in g v1 -> ~ edge_in g v1 v.
+
+Definition is_root (g:Graph) (v:Node) : Prop :=
+    no_parent g v.
+
+Example one_has_noparent_in_one_line:
+    no_parent one_line 1.
+Proof.
+    unfold no_parent. firstorder. inversion H; subst; clear H. unfold not. intros. unfold one_line in H. unfold edge_in in H. simpl in H. destruct H. specialize (H0 []). firstorder.
+    inversion H; subst; clear H.
+    unfold not. intros. unfold one_line in H. unfold edge_in in H. destruct H. simpl in H. specialize (H0 [2]). firstorder. easy. lia.
+Qed.
+
+
 Lemma maximal_path_exists_in_dag:
-    forall g l , is_dag g -> (exists max_path, (is_path g max_path) /\ ((is_path g l) -> (length l <= length max_path ))).
+    forall g , is_dag g -> (exists max_path, forall l, (is_path g max_path) /\ ((is_path g l) -> (length l <= length max_path ))).
 Proof.
 Admitted.
 
@@ -388,10 +868,10 @@ Admitted.
 Theorem dag_has_atleast_one_root: 
     forall g, is_dag g -> (exists v, node_in g v /\ no_parent g v).
 Proof.
-    intros. firstorder. 
+    intros.  apply  maximal_path_exists_in_dag in H. destruct H. 
 Admitted.
 
-
+(* Forest *)
 
 Definition is_forest (g:Graph) : Prop :=
     is_dag g /\ (forall p1 p2 v, node_in g v -> (edge_in g p1 v -> edge_in g p2 v  -> p1 = p2)).
@@ -400,28 +880,34 @@ Example is_line_is_forest:
     is_forest one_line.
 Proof.
     split.
-    unfold is_dag. apply one_line_is_not_cyclic.
-    unfold one_line. simpl. unfold edge_in. intros. firstorder. inversion H; subst; clear H. unfold edge_in in H1. destruct p1.
+    unfold is_dag. 
+    (* apply one_line_is_not_cyclic. *)
+    unfold one_line. simpl. unfold edge_in. intros. firstorder. inversion H; subst; clear H. unfold edge_in in H1. 
+    (* destruct p1. *)
 Admitted.
 
 Definition is_connected_ind (g: Graph) : Prop :=
- forall u v, (not (u = v) /\ node_in g u /\ node_in g v) -> (is_reachable_ind g u v  \/ is_reachable_ind g v u).
+ forall u v, not (u = v) -> (is_reachable_walk g u v).
 
 
+(* Is Graph a Tree *)
 
 Definition is_tree (g: Graph):
-    is_forest g /\   g.
+    is_forest g /\ is_connected_ind g.
 
 
 
 Definition is_leaf (g:Graph) (v: Node) :Prop :=
     (node_in g v) /\ (In (v, []) g).
 
+(* The following theorem requires knowledge that a path of maximum length occurs in a dag *)
+Theorem dag_has_atleast_one_leaf: 
+    forall g, is_dag g -> (exists v, is_leaf g v).
+Proof.
+    (* Proof.
+    intros.  apply  maximal_path_exists_in_dag in H. destruct H. 
+Admitted. *)
+
 Proof.
 Admitted.
-
-
-Theorem tree_has_1_less_internal_nodes_than_leaves:
-    True.
-
 
